Add some more basic features to the language

LambdaGraph/Basic.lean
@@ -1,3 +1,72 @@
+/-- The type of an expression. -/
+inductive Ty where
+  | bot
+  | unit
+  | bool
+  | int
+  | fn (t₁ t₂ : Ty)
+  | prod (t₁ t₂ : Ty)
+
+class Denote (α : Type) (β : outParam Type) where
+  denote : α → β
+
+notation "⟦" x "⟧" => Denote.denote x
+
+inductive Op where
+  | add
+  | sub
+  | mul
+
+instance : Denote Op (Int → Int → Int) where
+  denote
+    | .add => (· + ·)
+    | .sub => (· - ·)
+    | .mul => (· * ·)
+
+inductive Cmp where
+  | eq
+  | ne
+  | le
+  | lt
+
+instance : Denote Cmp (Int → Int → Bool) where
+  denote
+    | .eq => (· = ·)
+    | .ne => (· ≠ ·)
+    | .le => (· ≤ ·)
+    | .lt => (· < ·)
+
+inductive Logic where
+  | and
+  | or
+  | xor
+
+instance : Denote Logic (Bool → Bool → Bool) where
+  denote
+    | .and => (· && ·)
+    | .or => (· || ·)
+    | .xor => (· ^^ ·)
+
+inductive Const where
+  | unit
+  | bool (b : Bool)
+  | int (x : Int)
+  | op (f : Op)
+  | cmp (f : Cmp)
+  | logic (f : Logic)
+
+def Const.ty : Const → Ty
+  | unit => .unit
+  | bool _ => .bool
+  | int _ => .int
+  | op _ => .fn (.prod .int .int) .int
+  | cmp _ => .fn (.prod .int .int) .bool
+  | logic _ => .fn (.prod .bool .bool) .bool
+
+inductive BinKind where
+  | app
+  | pair
+
 /--
 An expression.
 
@@ -8,9 +77,41 @@ does not contain a construct for unnamed lambdas.
 inductive Expr where
   | var (n : Nat)
   | fn (n : Nat)
-  | app (f e : Expr)
-  | bool (b : Bool)
+  | const (c : Const)
+  | bin (k : BinKind) (e₁ e₂ : Expr)
   | cond (c et ef : Expr)
+  | proj (e : Expr) (i : Fin 2)
+
+abbrev Expr.unit : Expr := .const .unit
+
+abbrev Expr.app (f e : Expr) : Expr := f.bin .app e
+
+abbrev Expr.pair (e₁ e₂ : Expr) : Expr := e₁.bin .pair e₂
+
+@[coe]
+def Expr.ofBool (b : Bool) : Expr := .const (.bool b)
+
+@[coe]
+def Expr.ofInt (x : Int) : Expr := .const (.int x)
+
+@[coe]
+def Expr.ofOp (f : Op) : Expr := .const (.op f)
+
+@[coe]
+def Expr.ofCmp (f : Cmp) : Expr := .const (.cmp f)
+
+@[coe]
+def Expr.ofLogic (f : Logic) : Expr := .const (.logic f)
+
+instance : Coe Bool Expr := ⟨Expr.ofBool⟩
+
+instance : Coe Int Expr := ⟨Expr.ofInt⟩
+
+instance : Coe Op Expr := ⟨Expr.ofOp⟩
+
+instance : Coe Cmp Expr := ⟨Expr.ofCmp⟩
+
+instance : Coe Logic Expr := ⟨Expr.ofLogic⟩
 
 /--
 A recursive call of a function with its own argument.
@@ -18,12 +119,6 @@ A recursive call of a function with its own argument.
 This is used during substitution as a temporary placeholder body.
 -/
 abbrev Expr.recurse (n : Nat) : Expr := (fn n).app (var n)
-
-/-- The type of an `Expr`. -/
-inductive Ty where
-  | bot
-  | bool
-  | fn (t₁ t₂ : Ty)
 
 /--
 A collection of labelled lambda terms.
@@ -76,7 +171,8 @@ structure Computation extends Program where
 /-- A fully reduced expression. -/
 inductive Expr.Value : Expr → Prop where
   | fn n : Value (.fn n)
-  | bool b : Value (.bool b)
+  | const c : Value (.const c)
+  | pair v₁ v₂ : Value v₁ → Value v₂ → Value (v₁.pair v₂)
 
 /--
 The typing relation on expressions.
@@ -88,11 +184,17 @@ well-typed if their labels are in bounds.
 inductive Expr.Types (p : Program) : Expr → Ty → Prop where
   | var (n : Nat) (_ : n < p.size) : Types p (var n) p.ty[n]
   | fn (n : Nat) (_ : n < p.size) : Types p (fn n) (p.ty[n].fn p.ret[n])
+  | const (c : Const) : Types p (.const c) c.ty
   | app (f e : Expr) (t₁ t₂ : Ty) :
     Types p f (t₁.fn t₂) → Types p e t₁ → Types p (f.app e) t₂
-  | bool (b : Bool) : Types p (bool b) .bool
+  | pair (e₁ e₂ : Expr) (t₁ t₂ : Ty) :
+    Types p e₁ t₁ → Types p e₂ t₂ → Types p (e₁.pair e₂) (.prod t₁ t₂)
   | cond (c et ef : Expr) (t : Ty) :
     Types p c .bool → Types p et t → Types p ef t → Types p (c.cond et ef) t
+  | proj0 (e : Expr) (t₁ t₂ : Ty) :
+    Types p e (.prod t₁ t₂) → Types p (e.proj 0) t₁
+  | proj1 (e : Expr) (t₁ t₂ : Ty) :
+    Types p e (.prod t₁ t₂) → Types p (e.proj 1) t₂
 
 notation:60 p:61 " ⊢ " e:61 " : " t:61 => Expr.Types p e t
 
@@ -118,16 +220,6 @@ structure Computation.Types (p : Computation) (t : Ty) : Prop where
 
 notation:60 "⊢ " p:61 " : " t:61 => Computation.Types p t
 
-theorem value_types_fn {p : Program} {v : Expr} {t₁ t₂ : Ty}
-    (h : p ⊢ v : t₁.fn t₂) : v.Value → ∃ n, v = .fn n
-  | .fn n => by simp
-  | .bool b => nomatch h
-
-theorem value_types_bool {p : Program} {v : Expr} (h : p ⊢ v : .bool) :
-    v.Value → ∃ b, v = .bool b
-  | .fn n => nomatch h
-  | .bool b => by simp
-
 /-- A kind of reference, either a variable or a function. -/
 inductive RefKind where
   | var
@@ -137,11 +229,18 @@ inductive RefKind where
 inductive Expr.Local (n : Nat) : RefKind → Expr → Prop where
   | var : (var n).Local n .var
   | fn : (fn n).Local n .fn
-  | appL (r : RefKind) (f e : Expr) : f.Local n r → (f.app e).Local n r
-  | appR (r : RefKind) (f e : Expr) : e.Local n r → (f.app e).Local n r
-  | condC (r : RefKind) (c et ef : Expr) : c.Local n r → (c.cond et ef).Local n r
-  | condT (r : RefKind) (c et ef : Expr) : et.Local n r → (c.cond et ef).Local n r
-  | condF (r : RefKind) (c et ef : Expr) : ef.Local n r → (c.cond et ef).Local n r
+  | binL (r : RefKind) (k : BinKind) (e₁ e₂ : Expr) :
+    e₁.Local n r → (e₁.bin k e₂).Local n r
+  | binR (r : RefKind) (k : BinKind) (e₁ e₂ : Expr) :
+    e₂.Local n r → (e₁.bin k e₂).Local n r
+  | condC (r : RefKind) (c et ef : Expr) :
+    c.Local n r → (c.cond et ef).Local n r
+  | condT (r : RefKind) (c et ef : Expr) :
+    et.Local n r → (c.cond et ef).Local n r
+  | condF (r : RefKind) (c et ef : Expr) :
+    ef.Local n r → (c.cond et ef).Local n r
+  | proj (r : RefKind) (e : Expr) (i : Fin 2) :
+    e.Local n r → (e.proj i).Local n r
 
 /-- A local variable in an expression. -/
 abbrev Expr.LocalVar (e : Expr) (n : Nat) : Prop := e.Local n .var
@@ -168,6 +267,27 @@ def Program.ValidRefs (p : Program) : Prop :=
 @[grind →]
 theorem Program.Types.validRefs {p : Program} (ht : ⊢ p) : p.ValidRefs :=
   fun _ hi => (ht hi).validRefs
+
+theorem Expr.value_types_fn {p : Program} {v : Expr} {t₁ t₂ : Ty}
+    (h : p ⊢ v : t₁.fn t₂) : v.Value → (∃ n, v = .fn n) ∨
+      (∃ f : Op, v = f) ∨ (∃ f : Cmp, v = f) ∨ (∃ f : Logic, v = f)
+  | .fn n => Or.inl ⟨n, rfl⟩
+  | .const (.op f) => Or.inr (Or.inl ⟨f, rfl⟩)
+  | .const (.cmp f) => Or.inr (Or.inr (Or.inl ⟨f, rfl⟩))
+  | .const (.logic f) => Or.inr (Or.inr (Or.inr ⟨f, rfl⟩))
+
+theorem Expr.value_types_bool {p : Program} {v : Expr} (h : p ⊢ v : .bool) :
+    v.Value → ∃ b : Bool, v = b
+  | .const (.bool b) => ⟨b, rfl⟩
+
+theorem Expr.value_types_int {p : Program} {v : Expr} (h : p ⊢ v : .int) :
+    v.Value → ∃ x : Int, v = x
+  | .const (.int x) => ⟨x, rfl⟩
+
+theorem Expr.value_types_prod {p : Program} {v : Expr} {t₁ t₂ : Ty}
+    (h : p ⊢ v : t₁.prod t₂) : v.Value →
+      ∃ v₁ v₂, v = .pair v₁ v₂ ∧ v₁.Value ∧ v₂.Value
+  | .pair v₁ v₂ hv₁ hv₂ => ⟨v₁, v₂, rfl, hv₁, hv₂⟩
 
 @[grind →]
 theorem Expr.lt_size_of_local {p : Program} {e : Expr} {n : Nat} {r : RefKind}
@@ -201,17 +321,17 @@ theorem Expr.local_fn_iff {m n : Nat} {r : RefKind} :
     subst hr
     constructor
 
+@[simp, grind .]
+theorem Expr.not_local_const {c : Const} {n : Nat} {r : RefKind} :
+    ¬(const c).Local n r := nofun
+
 @[simp, grind =]
-theorem Expr.local_app_iff {f e : Expr} {n : Nat} {r : RefKind} :
-    (f.app e).Local n r ↔ f.Local n r ∨ e.Local n r := by
+theorem Expr.local_bin_iff {k : BinKind} {e₁ e₂ : Expr} {n : Nat} {r : RefKind} :
+    (e₁.bin k e₂).Local n r ↔ e₁.Local n r ∨ e₂.Local n r := by
   constructor
   · intro h
     cases h <;> solve_by_elim [Or.inl, Or.inr]
-  · rintro (hf | he) <;> solve_by_elim [Local.appL, Local.appR]
-
-@[simp, grind .]
-theorem Expr.not_local_bool {b : Bool} {n : Nat} {r : RefKind} :
-    ¬(bool b).Local n r := nofun
+  · rintro (h₁ | h₂) <;> solve_by_elim [Local.binL, Local.binR]
 
 @[simp, grind =]
 theorem Expr.local_cond_iff {c et ef : Expr} {n : Nat} {r : RefKind} :
@@ -221,6 +341,15 @@ theorem Expr.local_cond_iff {c et ef : Expr} {n : Nat} {r : RefKind} :
     cases h <;> solve_by_elim [Or.inl, Or.inr]
   · rintro (hc | het | hef) <;>
       solve_by_elim [Local.condC, Local.condT, Local.condF]
+
+@[simp, grind =]
+theorem Expr.local_proj_iff {e : Expr} {i : Fin 2} {n : Nat} {r : RefKind} :
+    (e.proj i).Local n r ↔ e.Local n r := by
+  constructor
+  · intro h
+    let .proj _ _ _ h := h
+    exact h
+  · exact .proj _ _ _
 
 @[simp, grind =]
 theorem Expr.bounded_var_iff {n m : Nat} :
@@ -240,24 +369,24 @@ theorem Expr.bounded_fn_iff {n m : Nat} :
     have .fn := hl
     exact h
 
+@[simp, grind .]
+theorem Expr.bounded_const {n : Nat} {c : Const} :
+    (const c).Bounded n := by
+  intro n r hl
+  cases hl
+
 @[simp, grind =]
-theorem Expr.bounded_app_iff {n : Nat} {f e : Expr} :
-    (f.app e).Bounded n ↔ f.Bounded n ∧ e.Bounded n := by
+theorem Expr.bounded_bin_iff {n : Nat} {k : BinKind} {e₁ e₂ : Expr} :
+    (e₁.bin k e₂).Bounded n ↔ e₁.Bounded n ∧ e₂.Bounded n := by
   constructor
   · intro h
     and_intros
     · intro m r hl
-      apply_rules [Local.appL]
+      apply_rules [Local.binL]
     · intro m r hl
-      apply_rules [Local.appR]
-  · intro ⟨hf, he⟩ m r hl
+      apply_rules [Local.binR]
+  · intro ⟨h₁, h₂⟩ m r hl
     cases hl <;> solve_by_elim
-
-@[simp, grind .]
-theorem Expr.bounded_bool {n : Nat} {b : Bool} :
-    (bool b).Bounded n := by
-  intro n r hl
-  cases hl
 
 @[simp, grind =]
 theorem Expr.bounded_cond_iff {n : Nat} {c et ef : Expr} :
@@ -273,6 +402,16 @@ theorem Expr.bounded_cond_iff {n : Nat} {c et ef : Expr} :
       apply_rules [Local.condF]
   · intro ⟨hc, het, hef⟩ m r hl
     cases hl <;> solve_by_elim
+
+@[simp, grind =]
+theorem Expr.bounded_proj_iff {n : Nat} {e : Expr} {i : Fin 2} :
+    (e.proj i).Bounded n ↔ e.Bounded n := by
+  constructor
+  · intro h m r hl
+    exact h (.proj _ _ _ hl)
+  · intro h m r hl
+    have .proj _ _ _ hl := hl
+    exact h hl
 
 @[grind .]
 theorem Expr.bounded_of_ge {n₁ n₂ : Nat} {e : Expr}
